examples/dm4free/FStar.DM4F.StExnC.fst
@@ -48,7 +48,7 @@ reifiable new_effect_for_free {
 }
 
 (* A lift from Pure *)
-inline let lift_pure_stexnc (a:Type) (wp:pure_wp a) (h0:int) (p:STEXNC.post a) =
+unfold let lift_pure_stexnc (a:Type) (wp:pure_wp a) (h0:int) (p:STEXNC.post a) =
         wp (fun a -> p (Some a, (h0, 0)))
 sub_effect PURE ~> STEXNC = lift_pure_stexnc
 
